modified ptr_eq to only be True for pointers (not all equal ints)

floyd/assert_lemmas.v
@@ -1079,7 +1079,7 @@ Qed.
 
 Definition ptr_eq (v1 v2: val) : Prop :=
       match v1,v2 with
-      | Vint n1, Vint n2 => Int.cmpu Ceq n1 n2 = true
+      | Vint n1, Vint n2 =>  Int.cmpu Ceq n1 n2 = true  /\ Int.cmpu Ceq n1 (Int.repr 0) = true
       | Vptr b1 ofs1,  Vptr b2 ofs2  =>
             b1=b2 /\ Int.cmpu Ceq ofs1 ofs2 = true
       | _,_ => False
@@ -1090,7 +1090,8 @@ Definition ptr_neq (v1 v2: val) := ~ ptr_eq v1 v2.
 Lemma ptr_eq_e: forall v1 v2, ptr_eq v1 v2 -> v1=v2.
 Proof.
 intros. destruct v1; destruct v2; simpl in H; try contradiction.
-pose proof (Int.eq_spec i i0). rewrite H in H0. subst; auto.
+pose proof (Int.eq_spec i i0). destruct H. 
+rewrite H in H0. subst; auto.
 destruct H; subst.
 f_equal.
 pose proof (Int.eq_spec i i0). rewrite H0 in H; auto.
